\documentclass{ximera}

\title{Algebra}

\begin{document}
\maketitle

\textbf{Question 14.} Multiplying the first equation by 3 and the second one by 2, we'll get the following equivalent system:
\begin{alignat*}{2}
 -6  x_1  + 12  x_2 & = -18 \\
 6  x_1  - 18  x_2 & = 24
\end{alignat*}
By summing these two equations we'll get $x_2 = -1$, and by replacing this value for $x_2$ in any of the equations, we'll obtain $x_1 = 1$.

\textbf{Question 15.} This is the formula for multiplication of two matrices $A_{m \times n}$ and $B_{n \times p}$:
\begin{equation*}
    (AB)_{ij} = \sum_{k=1}^n A_{ik}B_{kj}. 
\end{equation*}
Using this formula, we could compute the multiplication of the two given matrices:
\begin{equation*}
\begin{pmatrix}
8 & 12 & 7 \\
21 & 33 & 18 \\
28 & 36 & 26
\end{pmatrix}
\end{equation*}

\end{document}
